generational/spec/GC.Gen.Promote.fst
@@ -149,6 +149,21 @@ let promote_object (minor: minor_state) (major: heap) (obj: U64.t)
     let final_major = copy_fields minor new_major obj new_addr 0 wosize in
     { major_out = final_major; fp_out = new_fp; new_addr = new_addr }
 
+let promote_object_oom (minor: minor_state) (major: heap) (obj: U64.t)
+                       (fp: U64.t) (wosize: nat{wosize > 0})
+  : Lemma (requires (GC.Spec.Allocator.alloc_spec major fp wosize).obj_out == 0UL)
+          (ensures (let res = promote_object minor major obj fp wosize in
+                    res.major_out == major /\ res.fp_out == fp /\ res.new_addr == 0UL)) = ()
+
+let promote_object_success (minor: minor_state) (major: heap) (obj: U64.t)
+                           (fp: U64.t) (wosize: nat{wosize > 0})
+  : Lemma (requires (GC.Spec.Allocator.alloc_spec major fp wosize).obj_out <> 0UL)
+          (ensures (let alloc_res = GC.Spec.Allocator.alloc_spec major fp wosize in
+                    let res = promote_object minor major obj fp wosize in
+                    res.major_out == copy_fields minor alloc_res.heap_out obj alloc_res.obj_out 0 wosize /\
+                    res.fp_out == alloc_res.fp_out /\
+                    res.new_addr == alloc_res.obj_out)) = ()
+
 /// ---------------------------------------------------------------------------
 /// Promote all live objects
 /// ---------------------------------------------------------------------------
